reformulated lfill to enforce const in definition of lholed contexts instead

theories/operations.v
@@ -573,19 +573,16 @@ Definition result_to_stack (r : result) :=
   | result_trap => [:: AI_trap]
   end.
 
-Fixpoint lfill (k : nat) (lh : lholed) (es : seq administrative_instruction) : option (seq administrative_instruction) :=
+Fixpoint lfill (k : nat) (lh : lholed) (es : list administrative_instruction) : option (list administrative_instruction) :=
   match k with
   | 0 =>
-    if lh is LH_base vs es' then
-      if const_list vs then Some (app vs (app es es')) else None
+    if lh is LH_base vs es' then Some (app (v_to_e_list vs) (app es es'))
     else None
   | k'.+1 =>
-    if lh is LH_rec vs n es' lh' es'' then
-      if const_list vs then
+      if lh is LH_rec vs n es' lh' es'' then
         if lfill k' lh' es is Some lfilledk then
-          Some (app vs (cons (AI_label n es' lfilledk) es''))
-        else None
-      else None
+          Some (app (v_to_e_list vs) (cons (AI_label n es' lfilledk) es''))
+            else None
     else None
   end.
 
@@ -594,12 +591,10 @@ Definition lfilled (k : nat) (lh : lholed) (es : seq administrative_instruction)
 
 Inductive lfilledInd : nat -> lholed -> seq administrative_instruction -> seq administrative_instruction -> Prop :=
 | LfilledBase: forall vs es es',
-    const_list vs ->
-    lfilledInd 0 (LH_base vs es') es (vs ++ es ++ es')
+    lfilledInd 0 (LH_base vs es') es (v_to_e_list vs ++ es ++ es')
 | LfilledRec: forall k vs n es' lh' es'' es LI,
-    const_list vs ->
     lfilledInd k lh' es LI ->
-    lfilledInd (k.+1) (LH_rec vs n es' lh' es'') es (vs ++ [ :: (AI_label n es' LI) ] ++ es'').
+    lfilledInd (k.+1) (LH_rec vs n es' lh' es'') es (v_to_e_list vs ++ [ :: (AI_label n es' LI) ] ++ es'').
 
 Lemma lfilled_Ind_Equivalent: forall k lh es LI,
     lfilled k lh es LI <-> lfilledInd k lh es LI.
@@ -607,23 +602,21 @@ Proof.
   move => k. split.
   - move: lh es LI. induction k; move => lh es LI HFix.
     + unfold lfilled in HFix. simpl in HFix. destruct lh => //=.
-      * destruct (const_list l) eqn:HConst => //=.
-        { replace LI with (l++es++l0); first by apply LfilledBase.
-          symmetry. move: HFix. by apply/eqseqP. }
+      * replace LI with (v_to_e_list l++es++l0); first by apply LfilledBase.
+        symmetry. move: HFix. by apply/eqseqP.
     + unfold lfilled in HFix. simpl in HFix. destruct lh => //=.
-      * destruct (const_list l) eqn:HConst => //=.
-        { destruct (lfill k lh es) eqn:HLF => //=.
-          { replace LI with (l ++ [ :: (AI_label n l0 l2)] ++ l1).
-          apply LfilledRec; first by [].
+      * { destruct (lfill k lh es) eqn:HLF => //=.
+          { replace LI with (v_to_e_list l ++ [ :: (AI_label n l0 l2)] ++ l1).
+          apply LfilledRec.
           apply IHk. unfold lfilled; first by rewrite HLF.
           symmetry. move: HFix. by apply/eqseqP. }
         }
   - move => HLF. induction HLF.
-    + unfold lfilled. unfold lfill. by rewrite H.
-    + unfold lfilled. unfold lfill. rewrite H. fold lfill.
-      unfold lfilled in IHHLF. destruct (lfill k lh' es) => //=.
-      * replace LI with l => //=.
-        symmetry. by apply/eqseqP.
+    + unfold lfilled. unfold lfill. by apply/eqP.
+    + unfold lfilled. 
+      unfold lfilled in IHHLF => /=. destruct (lfill k lh' es) => //=.
+      * move/eqP in IHHLF; subst.
+        by apply/eqP.
 Qed.
 
 Lemma lfilledP: forall k lh es LI,
@@ -634,23 +627,6 @@ Proof.
   - apply ReflectF. move=> HContra. apply lfilled_Ind_Equivalent in HContra.
     by rewrite HLFBool in HContra.
 Qed.
-
-Fixpoint lfill_exact (k : nat) (lh : lholed) (es : seq administrative_instruction) : option (seq administrative_instruction) :=
-  match k with
-  | 0 =>
-    if lh is LH_base nil nil then Some es else None
-  | k'.+1 =>
-    if lh is LH_rec vs n es' lh' es'' then
-      if const_list vs then
-        if lfill_exact k' lh' es is Some lfilledk then
-          Some (app vs (cons (AI_label n es' lfilledk) es''))
-        else None
-      else None
-    else None
-  end.
-
-Definition lfilled_exact (k : nat) (lh : lholed) (es : seq administrative_instruction) (es' : seq administrative_instruction) : bool :=
-  if lfill_exact k lh es is Some es'' then es' == es'' else false.
 
 Definition result_types_agree (ts : result_type) r :=
   match r with
