theories/interp_instantiate_sound.v
@@ -355,15 +355,14 @@ Proof.
     move/lfilledP in H0.
     inversion H; inversion H0; subst; clear H; clear H0; try by destruct k0.
     2: { by do 2 destruct vs as [| ? vs] => //. }
-    injection H8 as ->; subst.
-    destruct vs as [ | a ?] => //; last by destruct a; try by destruct b => //.
-    destruct es, es'; simpl in *; subst => //.
+    injection H6 as ->; subst.
+    destruct vs, es, es' => //; simpl in *; subst => //.
     { by destruct es'. }
     { by destruct es. }
     destruct es, es', es'0 => //.
     simpl in *.
-    injection H1 as ->.
-    injection H6 as ->.
+    injection H5 as ->.
+    injection H9 as ->.
     by apply IHHred.
 Qed.
 
